formal/CclFormal.lean
@@ -7,5 +7,4 @@ import CclFormal.Decide
 import CclFormal.Json
 import CclFormal.Props
 import CclFormal.Equiv
-import CclFormal.Trans
 import CclFormal.Transitivity
